CTree/SemanticEquiv.lean
@@ -1,22 +1,78 @@
 import CTree.Euttc
 import CTree.LTS
+import CTree.ParLemmas
+import CTree.RefineSimLemmas
 
 namespace CTree
 
   theorem refine_of_weak_sim {sim : Rel (CTree ε ρ) (CTree ε ρ)} {t1 t2 : CTree ε ρ}
-    (hsim : IsWeakBisimulation sim) (h : sim t1 t2)
+    (hsim : IsWeakSimulation sim) (h : sim t1 t2)
     : t1 ≤Eq≤ t2 := by
-    sorry
+    apply Refine.coind (λ p1 p2 t1 t2 => sim t1 t2) _ 0 0 h
+    intro p1 p2 t1 t2 h
+    apply dMatchOn t1
+    · intro x heq
+      subst heq
+      apply dMatchOn t2
+      · intro y heq
+        subst heq
+        have := hsim (ret x) (ret y) h (.val x) zero .ret
+        simp only at this
+        obtain ⟨t2', hws, h⟩ := this
+        apply RefineF.ret
+        symm
+        exact hws.ret_val
+      · intro c heq
+        subst heq
+        sorry
+      · sorry
+      · sorry
+      · sorry
+    · sorry
+    · sorry
+    · sorry
+    · sorry
 
-  theorem euttc_of_lts {t1 t2 : CTree ε ρ} (h : WeakBisim t1 t2) : t1 ≈ t2 := by
+  theorem euttc_of_weak_bisim {t1 t2 : CTree ε ρ} (h : WeakBisim t1 t2) : t1 ≈ t2 := by
     obtain ⟨sim, ⟨⟨hsim1, hsim2⟩, h⟩⟩ := h
+    apply And.intro
+    · exact refine_of_weak_sim hsim1 h
+    · rw [flip_eq]
+      exact refine_of_weak_sim hsim2 h
 
+  theorem weak_sim_of_refine : IsWeakSimulation (Refine Eq (ρ := ρ) (ε := ε)) := by
+    intro t1 t2 href l t1' hs
+    obtain ⟨_, _, href⟩ := href
+    split
+    · have := refine_tau_correspondence href t1' hs
+      exists 0, t2
+      apply And.intro rfl
+      rename_i p1 p2 _
+      exists p1, p2
+    · cases l with
+      | tau => contradiction
+      | val v =>
+        have := Step.zero_of_val hs
+        subst this
+        have := refine_ret_correspondence href hs
+        have := weak_step_of_refine_ret this
+        exists zero
+        exact And.intro this Refine.zero_le
+      | event =>
+        have ⟨t2', hws, href⟩ := refine_event_correspondence href _ hs
+        exists t2'
+        exact And.intro hws ⟨_, _, href⟩
+
+  theorem weak_bisim_of_euttc {t1 t2 : CTree ε ρ} (h : t1 ≈ t2) : WeakBisim t1 t2 := by
+    exists Refine Eq
+    apply And.intro
+    · apply And.intro weak_sim_of_refine
+      -- Cannot prove the reverse is also a simulation,
+      -- because a choice only needs to refine one side in the reverse
+      sorry
     sorry
 
-  theorem lts_of_euttc {t1 t2 : CTree ε ρ} (h : t1 ≈ t2) : WeakBisim t1 t2 := by
-    sorry
-
-  theorem euttc_iff_lts {t1 t2 : CTree ε ρ} : t1 ≈ t2 ↔ WeakBisim t1 t2 :=
-    ⟨lts_of_euttc, euttc_of_lts⟩
+  theorem euttc_iff_weak_bisim {t1 t2 : CTree ε ρ} : t1 ≈ t2 ↔ WeakBisim t1 t2 :=
+    ⟨weak_bisim_of_euttc, euttc_of_weak_bisim⟩
 
 end CTree
